supp -> finsupp.

theories/ffun.v
@@ -9,7 +9,7 @@ From extructures Require Import ord fset fmap.
 (* on all but finitely many inputs.  The type T must be an instance of        *)
 (* ordType, and S must be an eqType.                                          *)
 (*                                                                            *)
-(*        supp f == the finite set of inputs where f differs from def         *)
+(*     finsupp f == the finite set of inputs where f differs from def         *)
 (*   mkffun f xs == the finite function defined by                            *)
 (*                      mkffun f xs x = if x \in xs then f x else def x       *)
 (*     mkffunm m == complete a finite map m with def outside of the domain    *)
@@ -62,21 +62,21 @@ case efx: (val f x)=> [y1|]; case egx: (val g x)=> [y2|] // e.
   by move: (allP (valP g) _ xP); rewrite egx e eqxx.
 Qed.
 
-Definition supp f := domm (val f).
+Definition finsupp f := domm (val f).
 
-Lemma mem_supp f x : (x \in supp f) = (f x != def x).
+Lemma mem_finsupp f x : (x \in finsupp f) = (f x != def x).
 Proof.
-rewrite /appf /supp mem_domm.
+rewrite /appf /finsupp mem_domm.
 case efx: (val f x)=> [y|]; last by rewrite eqxx.
 have xP: x \in domm (val f) by rewrite mem_domm efx.
 by move: (allP (valP f) _ xP); rewrite efx => ->.
 Qed.
 
-Lemma mem_suppN f x : (x \notin supp f) = (f x == def x).
-Proof. by rewrite mem_supp negbK. Qed.
+Lemma mem_finsuppN f x : (x \notin finsupp f) = (f x == def x).
+Proof. by rewrite mem_finsupp negbK. Qed.
 
-Lemma suppPn f x : reflect (f x = def x) (x \notin supp f).
-Proof. rewrite mem_supp negbK; exact/eqP. Qed.
+Lemma finsuppPn f x : reflect (f x = def x) (x \notin finsupp f).
+Proof. rewrite mem_finsupp negbK; exact/eqP. Qed.
 
 Lemma emptyf_subproof : wf (@emptym T S).
 Proof. by rewrite domm0. Qed.
@@ -86,7 +86,7 @@ Definition emptyf := FFun emptym emptyf_subproof.
 Lemma emptyfE x : emptyf x = def x.
 Proof. by []. Qed.
 
-Lemma supp0 : supp emptyf = fset0.
+Lemma finsupp0 : finsupp emptyf = fset0.
 Proof. exact/domm0. Qed.
 
 Definition upd_def f x y :=
@@ -123,28 +123,28 @@ elim: xs=> [|x' xs IH] //=; rewrite inE updE IH.
 by case: eqP => [<-|_].
 Qed.
 
-Lemma supp_mkffun fb xs :
-  supp (mkffun fb xs) = fset [seq x <- xs | fb x != def x].
+Lemma finsupp_mkffun fb xs :
+  finsupp (mkffun fb xs) = fset [seq x <- xs | fb x != def x].
 Proof.
-apply/eq_fset=> x; rewrite mem_supp in_fset mem_filter mkffunE.
+apply/eq_fset=> x; rewrite mem_finsupp in_fset mem_filter mkffunE.
 by rewrite andbC; case: ifP=> //; rewrite eqxx.
 Qed.
 
-Lemma supp_mkffun_sub fb (X : {fset T}) : supp (mkffun fb X) `<=` X.
+Lemma finsupp_mkffun_sub fb (X : {fset T}) : finsupp (mkffun fb X) `<=` X.
 Proof.
-by apply/fsubsetP => x; rewrite supp_mkffun in_fset mem_filter; case/andP.
+by apply/fsubsetP => x; rewrite finsupp_mkffun in_fset mem_filter; case/andP.
 Qed.
 
 Definition updfm f (xs : {fmap T -> S}) : ffun :=
   mkffun (fun v => if xs v is Some x then x else f v)
-         (supp f `|` domm xs).
+         (finsupp f `|` domm xs).
 
 Lemma updfmE f xs x :
   updfm f xs x = if xs x is Some y then y else f x.
 Proof.
 rewrite /updm mkffunE in_fsetU orbC mem_domm.
 case e: (xs x)=> [y|] //=.
-by case: ifPn=> // /suppPn ->.
+by case: ifPn=> // /finsuppPn ->.
 Qed.
 
 Definition mkffunm (m : {fmap T -> S}) : ffun :=
@@ -171,19 +171,19 @@ Qed.
 End FFun.
 
 Arguments ffun {T S} def.
-Arguments suppPn {T S def f x}.
+Arguments finsuppPn {T S def f x}.
 
 Section Mapping.
 
 Variables (T : ordType) (S R : eqType) (def : T -> S).
 
 Definition mapf (g : S -> R) (f : ffun def) : ffun (g \o def) :=
-  mkffun (g \o f) (supp f).
+  mkffun (g \o f) (finsupp f).
 
 Lemma mapfE (g : S -> R) (f : ffun def) x :
   mapf g f x = g (f x).
 Proof.
-rewrite /mapf mkffunE mem_supp /=.
+rewrite /mapf mkffunE mem_finsupp /=.
 by case: eqP=> //= ->.
 Qed.
 
@@ -192,7 +192,7 @@ Lemma val_mapf (g : S -> R) :
   forall f : ffun def, ffval (mapf g f) = mapm g (ffval f).
 Proof.
 move=> g_inj f; apply/eq_fmap=> x.
-rewrite /mapf val_mkffun mkfmapfpE mapmE mem_supp /= /appf /=.
+rewrite /mapf val_mkffun mkfmapfpE mapmE mem_finsupp /= /appf /=.
 rewrite inj_eq //.
 case e: (ffval f x)=> [y|] /=; last by rewrite eqxx.
 have xdomm: x \in domm (ffval f) by rewrite mem_domm e.
@@ -209,3 +209,18 @@ HB.instance Definition _ T (S : eqType) def :=
   [Choice of @ffun T S def by <:].
 #[hnf] HB.instance Definition _ T (S : ordType) def :=
   [Ord of @ffun T S def by <:].
+
+#[deprecated(since="extructures 0.6.0", note="use finsupp instead")]
+Notation supp := finsupp (only parsing).
+#[deprecated(since="extructures 0.6.0", note="use mem_finsupp instead")]
+Notation mem_supp := mem_finsupp (only parsing).
+#[deprecated(since="extructures 0.6.0", note="use mem_finsuppN instead")]
+Notation mem_suppN := mem_finsuppN (only parsing).
+#[deprecated(since="extructures 0.6.0", note="use finsuppPn instead")]
+Notation suppPn := finsuppPn (only parsing).
+#[deprecated(since="extructures 0.6.0", note="use finsupp0 instead")]
+Notation supp0 := finsupp0 (only parsing).
+#[deprecated(since="extructures 0.6.0", note="use finsupp_mkffun instead")]
+Notation supp_mkffun := finsupp_mkffun (only parsing).
+#[deprecated(since="extructures 0.6.0", note="use finsupp_mkffun_sub instead")]
+Notation supp_mkffun_sub := finsupp_mkffun_sub (only parsing).
