theories/fperm.v
@@ -11,7 +11,7 @@ Require Import ord fset fmap ffun.
 (* and thus support extensional equality (cf. eq_fperm).                      *)
 (*                                                                            *)
 (*         fperm_one, 1 == Identity permutation.                              *)
-(*               supp s == The support of s (the set of elements that are not *)
+(*            finsupp s == The support of s (the set of elements that are not *)
 (*                         fixed by s).                                       *)
 (*            fperm f X == Builds a permutation out of a function f.  If f is *)
 (*                         bijective on X and x \in X, then fperm f X x = f x *)
@@ -36,7 +36,7 @@ Variables (T : ordType).
 Local Open Scope ord_scope.
 Local Open Scope fset_scope.
 
-Definition axiom (f : ffun (@id T)) := f @` supp f == supp f.
+Definition axiom (f : ffun (@id T)) := f @` finsupp f == finsupp f.
 
 Record fperm_type := FPerm {
   fpval : ffun id;
@@ -90,35 +90,35 @@ Proof.
 split; last congruence; by move=> /eq_ffun /val_inj.
 Qed.
 
-Lemma imfset_supp s : s @` supp s = supp s.
+Lemma imfset_finsupp s : s @` finsupp s = finsupp s.
 Proof. exact/eqP/(valP s). Qed.
 
-Lemma imfset_suppS s X : supp s `<=` X -> s @` X = X.
+Lemma imfset_finsuppS s X : finsupp s `<=` X -> s @` X = X.
 Proof.
-move=> subX; rewrite -(fsetID X (supp s)) imfsetU.
-rewrite (fsetIidPr subX) imfset_supp; congr fsetU.
-under eq_in_imfset => x /fsetDP [] _ /suppPn -> do [].
+move=> subX; rewrite -(fsetID X (finsupp s)) imfsetU.
+rewrite (fsetIidPr subX) imfset_finsupp; congr fsetU.
+under eq_in_imfset => x /fsetDP [] _ /finsuppPn -> do [].
 by rewrite imfset_id.
 Qed.
 
 Lemma fperm_inj s : injective s.
 Proof.
 move=> x y.
-have inj : {in x |` (y |` supp s) &, injective s}.
-  apply/imfset_injP; rewrite imfset_suppS //.
+have inj : {in x |` (y |` finsupp s) &, injective s}.
+  apply/imfset_injP; rewrite imfset_finsuppS //.
   by rewrite fsubsetU // fsubsetU ?fsubsetxx orbT.
 by apply: inj; rewrite ?in_fsetU1 ?eqxx // ?orbT.
 Qed.
 
-Lemma fperm_supp s x : (s x \in supp s) = (x \in supp s).
+Lemma fperm_finsupp s x : (s x \in finsupp s) = (x \in finsupp s).
 Proof.
-rewrite -{1}imfset_supp; apply/(sameP idP)/(iffP idP).
+rewrite -{1}imfset_finsupp; apply/(sameP idP)/(iffP idP).
   by apply: mem_imfset.
 by case/imfsetP=> x' hx' /fperm_inj ->.
 Qed.
 
 Lemma fperm_one_subproof : FPerm.axiom (@emptyf T _ _).
-Proof. by rewrite /FPerm.axiom supp0 imfset0. Qed.
+Proof. by rewrite /FPerm.axiom finsupp0 imfset0. Qed.
 
 Definition fperm_one : {fperm T} :=
   @FPerm.FPerm T emptyf fperm_one_subproof.
@@ -128,32 +128,28 @@ Lemma fperm1 x : 1 x = x.
 Proof. by []. Qed.
 
 
-Lemma mem_suppN s x : (x \notin supp s) = (s x == x).
-Proof. by rewrite mem_supp negbK. Qed.
-
-
-Lemma imfset_supp_sub s X : supp s `<=` X -> s @` X = X.
+Lemma imfset_finsupp_sub s X : finsupp s `<=` X -> s @` X = X.
 Proof.
 move=> h_sub; apply/eq_fset=> x; have h_im_sub := imfsetS s h_sub.
-have [in_supp|nin_supp] := boolP (x \in supp s).
-  rewrite (fsubsetP h_sub _ in_supp); move/fsubsetP: h_im_sub; apply.
-  by rewrite imfset_supp.
-move: nin_supp; rewrite mem_supp negbK =>/eqP ex.
+have [in_finsupp|nin_finsupp] := boolP (x \in finsupp s).
+  rewrite (fsubsetP h_sub _ in_finsupp); move/fsubsetP: h_im_sub; apply.
+  by rewrite imfset_finsupp.
+move: nin_finsupp; rewrite mem_finsupp negbK =>/eqP ex.
 apply/(sameP idP)/(iffP idP); first by rewrite -{2}ex; apply: mem_imfset.
 case/imfsetP=> [y Py ey]; rewrite {2}ey in ex.
 by move/fperm_inj in ex; rewrite ex.
 Qed.
 
-Lemma supp1 : supp 1 = fset0.
+Lemma finsupp1 : finsupp 1 = fset0.
 Proof.
 apply/eqP; rewrite -fsubset0; apply/fsubsetP=> x.
-by rewrite mem_supp fperm1 eqxx.
+by rewrite mem_finsupp fperm1 eqxx.
 Qed.
 
-Lemma supp_eq0 s : (supp s == fset0) = (s == 1).
+Lemma finsupp_eq0 s : (finsupp s == fset0) = (s == 1).
 Proof.
-apply/(sameP idP)/(iffP idP)=> [/eqP->|]; first by rewrite supp1.
-move=> /eqP e; apply/eqP/eq_fperm=> x; rewrite fperm1; apply/suppPn.
+apply/(sameP idP)/(iffP idP)=> [/eqP->|]; first by rewrite finsupp1.
+move=> /eqP e; apply/eqP/eq_fperm=> x; rewrite fperm1; apply/finsuppPn.
 by rewrite e in_fset0.
 Qed.
 
@@ -164,13 +160,13 @@ Implicit Types (f : T -> T).
 Lemma fperm_def_aux f X : f @` X = X -> FPerm.axiom (mkffun f X).
 Proof.
 move=> fP; apply/eqP/eq_fset => x; apply/(sameP idP)/(iffP idP).
-- rewrite {1}supp_mkffun in_fset mem_filter; case/andP => fx_x x_X.
+- rewrite {1}finsupp_mkffun in_fset mem_filter; case/andP => fx_x x_X.
   move: x x_X fx_x; rewrite -{1}fP => _ /imfsetP [] x x_X -> ffx_fx.
   apply/imfsetP; exists x.
-    by rewrite mem_supp mkffunE x_X; apply: contraNN ffx_fx => /eqP {1}->.
+    by rewrite mem_finsupp mkffunE x_X; apply: contraNN ffx_fx => /eqP {1}->.
   by rewrite mkffunE x_X.
 - case/imfsetP => {}x x_X ->.
-  move: x_X; rewrite !mem_supp !mkffunE.
+  move: x_X; rewrite !mem_finsupp !mkffunE.
   case: ifP => [x_X fx_x|]; last by rewrite eqxx.
   have fx_X : f x \in X by rewrite -fP mem_imfset.
   have inj : {in X &, injective f} by apply/imfset_injP; rewrite fP.
@@ -221,18 +217,18 @@ rewrite /g; case: ifPn => x_Y1; last first.
 by case/fsetDP: (nth_Y2 _ x_X x_Y1) => ? ?; apply/fsetUP; left.
 Qed.
 
-Lemma supp_fperm f X : supp (fperm f X) `<=` X `|` f @` X.
+Lemma finsupp_fperm f X : finsupp (fperm f X) `<=` X `|` f @` X.
 Proof.
-rewrite /fperm; case: insubP => /= [g _ ->|_]; first exact: supp_mkffun_sub.
-by rewrite supp0 fsub0set.
+rewrite /fperm; case: insubP => /= [g _ ->|_]; first exact: finsupp_mkffun_sub.
+by rewrite finsupp0 fsub0set.
 Qed.
 
 Lemma fpermEst f X x : f @` X = X -> fperm f X x = if x \in X then f x else x.
 Proof.
 move=> st; case: ifPn=> /= [|x_nin].
   by apply/fpermE/imfset_injP/eqP; rewrite st.
-apply/suppPn; apply: contra x_nin; apply/fsubsetP.
-rewrite -{2}[X]fsetUid -{3}st; exact: supp_fperm.
+apply/finsuppPn; apply: contra x_nin; apply/fsubsetP.
+rewrite -{2}[X]fsetUid -{3}st; exact: finsupp_fperm.
 Qed.
 
 End Build.
@@ -242,12 +238,12 @@ Section Renaming.
 (* FIXME: find a better name for this *)
 Lemma find_fperm (X Y : {fset T}) :
   size X = size Y ->
-  exists2 s : {fperm T}, supp s `<=` X `|` Y & s @` X = Y.
+  exists2 s : {fperm T}, finsupp s `<=` X `|` Y & s @` X = Y.
 Proof.
 move=> size_X.
 suff [f f_inj im_f]: exists2 f, {in X &, injective f} & f @` X = Y.
   rewrite -im_f.
-  exists (fperm f X); first by rewrite supp_fperm.
+  exists (fperm f X); first by rewrite finsupp_fperm.
   by apply: eq_in_imfset; apply: fpermE.
 elim/fset_ind: X Y size_X => [|x X x_nin_X IH] Y.
   rewrite /=; move/esym/eqP; rewrite sizes_eq0=> /eqP ->.
@@ -277,58 +273,58 @@ Section Inverse.
 
 Variable s : {fperm T}.
 
-Local Notation inv_def := (fun x => odflt x (fpick (pred1 x \o s) (supp s))).
+Local Notation inv_def := (fun x => odflt x (fpick (pred1 x \o s) (finsupp s))).
 
-Lemma fperm_inv_subproof : inv_def @` supp s = supp s.
+Lemma fperm_inv_subproof : inv_def @` finsupp s = finsupp s.
 Proof.
 apply/eq_fset=> x; apply/(sameP idP)/(iffP idP).
-  move=> x_in_supp; apply/imfsetP; exists (s x).
-    by rewrite -imfset_supp (mem_imfset _ x_in_supp).
-  case: fpickP=> [y' /= /eqP/esym e _|/(_ _ x_in_supp) /=].
+  move=> x_in_finsupp; apply/imfsetP; exists (s x).
+    by rewrite -imfset_finsupp (mem_imfset _ x_in_finsupp).
+  case: fpickP=> [y' /= /eqP/esym e _|/(_ _ x_in_finsupp) /=].
     exact: fperm_inj e.
   by rewrite eqxx.
 by case/imfsetP=> [y Py -> {x}]; case: fpickP.
 Qed.
 
-Definition fperm_inv := locked (fperm inv_def (supp s)).
+Definition fperm_inv := locked (fperm inv_def (finsupp s)).
 
 Lemma fpermK : cancel s fperm_inv.
 Proof.
 move=> x; rewrite /fperm_inv -lock fpermEst; last exact: fperm_inv_subproof.
-rewrite fperm_supp; case: ifPn=> [x_in_supp|]; last exact/suppPn.
-case: fpickP => [y /= /eqP/esym /fperm_inj-> //|/(_ _ x_in_supp) /=].
+rewrite fperm_finsupp; case: ifPn=> [x_in_finsupp|]; last exact/finsuppPn.
+case: fpickP => [y /= /eqP/esym /fperm_inj-> //|/(_ _ x_in_finsupp) /=].
 by rewrite eqxx.
 Qed.
 
 Lemma fpermKV : cancel fperm_inv s.
 Proof.
 move=> x; rewrite /fperm_inv -lock fpermEst; last exact: fperm_inv_subproof.
-case: ifPn=> [x_in_supp|].
+case: ifPn=> [x_in_finsupp|].
   case: fpickP=> [x' /= /eqP/esym -> //|/=].
-  rewrite -imfset_supp in x_in_supp; case/imfsetP: x_in_supp=> [x' Px' ->].
+  rewrite -imfset_finsupp in x_in_finsupp; case/imfsetP: x_in_finsupp=> [x' Px' ->].
   by move/(_ _ Px'); rewrite eqxx.
-by rewrite mem_supp negbK => /eqP.
+by rewrite mem_finsupp negbK => /eqP.
 Qed.
 
-Lemma supp_inv : supp fperm_inv = supp s.
+Lemma finsupp_inv : finsupp fperm_inv = finsupp s.
 Proof.
 apply/eq_fset=> x; apply/(sameP idP)/(iffP idP).
-  by rewrite !mem_supp; apply: contra => /eqP {1}<-; rewrite fpermKV eqxx.
-by rewrite !mem_supp; apply: contra=> /eqP {1}<-; rewrite fpermK eqxx.
+  by rewrite !mem_finsupp; apply: contra => /eqP {1}<-; rewrite fpermKV eqxx.
+by rewrite !mem_finsupp; apply: contra=> /eqP {1}<-; rewrite fpermK eqxx.
 Qed.
 
-Lemma fperm_suppV x : (fperm_inv x \in supp s) = (x \in supp s).
-Proof. by rewrite -{1}supp_inv fperm_supp supp_inv. Qed.
+Lemma fperm_finsuppV x : (fperm_inv x \in finsupp s) = (x \in finsupp s).
+Proof. by rewrite -{1}finsupp_inv fperm_finsupp finsupp_inv. Qed.
 
 End Inverse.
 
 Lemma fperm_mul_subproof s1 s2 :
-  (s1 \o s2) @` (supp s1 `|` supp s2) = supp s1 `|` supp s2.
+  (s1 \o s2) @` (finsupp s1 `|` finsupp s2) = finsupp s1 `|` finsupp s2.
 Proof.
-by rewrite imfset_comp !imfset_supp_sub // ?fsubsetUr // fsubsetUl.
+by rewrite imfset_comp !imfset_finsupp_sub // ?fsubsetUr // fsubsetUl.
 Qed.
 
-Definition fperm_mul s1 s2 := locked (fperm (s1 \o s2) (supp s1 `|` supp s2)).
+Definition fperm_mul s1 s2 := locked (fperm (s1 \o s2) (finsupp s1 `|` finsupp s2)).
 
 Infix "*" := fperm_mul.
 Notation "x ^-1" := (fperm_inv x).
@@ -336,45 +332,45 @@ Notation "x ^-1" := (fperm_inv x).
 Lemma fpermM s1 s2 : s1 * s2 =1 s1 \o s2.
 Proof.
 move=> x; rewrite /fperm_mul -lock fpermEst; last exact: fperm_mul_subproof.
-have [|nin_supp] //= := boolP (x \in _).
-rewrite in_fsetU negb_or !mem_supp !negbK in nin_supp.
-by case/andP: nin_supp=> [/eqP h1 /eqP ->]; rewrite h1.
+have [|nin_finsupp] //= := boolP (x \in _).
+rewrite in_fsetU negb_or !mem_finsupp !negbK in nin_finsupp.
+by case/andP: nin_finsupp=> [/eqP h1 /eqP ->]; rewrite h1.
 Qed.
 
-Lemma supp_mul s1 s2 : supp (s1 * s2) `<=` supp s1 `|` supp s2.
+Lemma finsupp_mul s1 s2 : finsupp (s1 * s2) `<=` finsupp s1 `|` finsupp s2.
 Proof.
-apply/fsubsetP=> x; rewrite in_fsetU !mem_supp fpermM /=.
+apply/fsubsetP=> x; rewrite in_fsetU !mem_finsupp fpermM /=.
 have [-> -> //|] := altP (s2 x =P x).
 by rewrite orbT.
 Qed.
 
-Lemma suppJ s1 s2 : supp (s1 * s2 * s1^-1) = s1 @` supp s2.
+Lemma finsuppJ s1 s2 : finsupp (s1 * s2 * s1^-1) = s1 @` finsupp s2.
 Proof.
-apply/eq_fset=> x; apply/esym/imfsetP; rewrite mem_supp fpermM /= fpermM /=.
+apply/eq_fset=> x; apply/esym/imfsetP; rewrite mem_finsupp fpermM /= fpermM /=.
 rewrite (can2_eq (fpermK s1) (fpermKV s1)).
 have [e|ne] /= := altP eqP.
   case=> [y Py e']; move: e Py.
-  by rewrite e' fpermK mem_supp=> ->; rewrite eqxx.
+  by rewrite e' fpermK mem_finsupp=> ->; rewrite eqxx.
 exists (s1^-1 x); last by rewrite fpermKV.
-by rewrite mem_supp.
+by rewrite mem_finsupp.
 Qed.
 
 Lemma fperm_mulC s1 s2 :
-  fdisjoint (supp s1) (supp s2) ->
+  fdisjoint (finsupp s1) (finsupp s2) ->
   s1 * s2 = s2 * s1.
 Proof.
 move=> dis; apply/eq_fperm=> x; rewrite !fpermM /=.
-have [ins1|nins1] := boolP (x \in supp s1).
-  move: (ins1); rewrite -fperm_supp=> ins1'.
+have [ins1|nins1] := boolP (x \in finsupp s1).
+  move: (ins1); rewrite -fperm_finsupp=> ins1'.
   move/fdisjointP in dis.
-  move/suppPn: (dis _ ins1)=> ->.
-  by move/suppPn: (dis _ ins1')=> ->.
-have [ins2|nins2] := boolP (x \in supp s2).
-  move: (ins2); rewrite -fperm_supp=> ins2'.
+  move/finsuppPn: (dis _ ins1)=> ->.
+  by move/finsuppPn: (dis _ ins1')=> ->.
+have [ins2|nins2] := boolP (x \in finsupp s2).
+  move: (ins2); rewrite -fperm_finsupp=> ins2'.
   move: dis; rewrite fdisjointC=> /fdisjointP dis.
-  move/suppPn: (dis _ ins2)=> ->.
-  by move/suppPn: (dis _ ins2')=> ->.
-move: nins1 nins2=> /suppPn nins1 /suppPn nins2.
+  move/finsuppPn: (dis _ ins2)=> ->.
+  by move/finsuppPn: (dis _ ins2')=> ->.
+move: nins1 nins2=> /finsuppPn nins1 /finsuppPn nins2.
 by rewrite nins1 nins2.
 Qed.
 
@@ -488,55 +484,55 @@ apply/eq_fperm=> y; rewrite fperm2E fperm1 /=.
 by have [->|] := altP (y =P x).
 Qed.
 
-Lemma supp_fperm2 x y :
-  supp (fperm2 x y) = if x == y then fset0 else [fset x; y].
+Lemma finsupp_fperm2 x y :
+  finsupp (fperm2 x y) = if x == y then fset0 else [fset x; y].
 Proof.
-have [<-{y}|ne] := altP eqP; first by rewrite fperm2xx supp1.
-apply/eq_fset=> z; rewrite mem_supp /= in_fset2.
+have [<-{y}|ne] := altP eqP; first by rewrite fperm2xx finsupp1.
+apply/eq_fset=> z; rewrite mem_finsupp /= in_fset2.
 case: fperm2P => [->|->|]; [rewrite eq_sym| |]; rewrite ?ne ?eqxx ?orbT //.
 by move=> /eqP/negbTE-> /eqP/negbTE->.
 Qed.
 
-Lemma fsubset_supp_fperm2 x y : supp (fperm2 x y) `<=` [fset x; y].
+Lemma fsubset_finsupp_fperm2 x y : finsupp (fperm2 x y) `<=` [fset x; y].
 Proof.
-by rewrite supp_fperm2 fun_if if_arg fsub0set fsubsetxx; case: (_ == _).
+by rewrite finsupp_fperm2 fun_if if_arg fsub0set fsubsetxx; case: (_ == _).
 Qed.
 
 Lemma fperm2_rect (P : {fperm T} -> Type) :
   P 1 ->
-  (forall x y s, x \notin supp s -> y \in supp (fperm2 x y * s) ->
+  (forall x y s, x \notin finsupp s -> y \in finsupp (fperm2 x y * s) ->
                  P s -> P (fperm2 x y * s)) ->
   forall s, P s.
 Proof.
-move=> P1 PM s; move: {2}(size _) (leqnn (size (supp s)))=> n.
-elim: n s=> [|n IH] s; first by rewrite leqn0 sizes_eq0 supp_eq0=> /eqP ->.
-case e: (supp s) / fsetP=>[|x X Px].
-  by move/eqP: e; rewrite supp_eq0=> /eqP ->.
+move=> P1 PM s; move: {2}(size _) (leqnn (size (finsupp s)))=> n.
+elim: n s=> [|n IH] s; first by rewrite leqn0 sizes_eq0 finsupp_eq0=> /eqP ->.
+case e: (finsupp s) / fsetP=>[|x X Px].
+  by move/eqP: e; rewrite finsupp_eq0=> /eqP ->.
 rewrite sizesU1 Px ltnS -(fperm_mulKs (fperm2 x (s x)) s) fperm2V=> es.
-apply: PM; first by apply/suppPn; rewrite fpermM /= fperm2R.
-  by rewrite -{1}fperm2V fperm_mulKs fperm_supp e in_fsetU1 eqxx.
+apply: PM; first by apply/finsuppPn; rewrite fpermM /= fperm2R.
+  by rewrite -{1}fperm2V fperm_mulKs fperm_finsupp e in_fsetU1 eqxx.
 apply: IH; rewrite (leq_trans _ es) // {es}; apply/fsubset_leq_size/fsubsetP.
-move=> y; rewrite mem_supp fpermM /=; case: fperm2P.
-- move=> ex ny; have: y \in supp s.
-    by have [//|/suppPn ey] := boolP (y \in _); rewrite -ex !ey eqxx in ny.
+move=> y; rewrite mem_finsupp fpermM /=; case: fperm2P.
+- move=> ex ny; have: y \in finsupp s.
+    by have [//|/finsuppPn ey] := boolP (y \in _); rewrite -ex !ey eqxx in ny.
   by rewrite e; case/fsetU1P=> [ey|//]; rewrite -ey ex ey eqxx in ny.
 - by move/fperm_inj=> ->; rewrite eqxx.
 move=> _ /eqP; rewrite (inj_eq (@fperm_inj _))=> e2.
-by rewrite -mem_supp e in_fsetU1 (negbTE e2).
+by rewrite -mem_finsupp e in_fsetU1 (negbTE e2).
 Qed.
 
 Definition enum_fperm X : {fset {fperm T}} :=
   fset (pmap (obind (insub : ffun _ -> option {fperm T}) \o insub)
           (enum_fmap X X)).
 
-Lemma enum_fpermE X s : supp s `<=` X = (s \in enum_fperm X).
+Lemma enum_fpermE X s : finsupp s `<=` X = (s \in enum_fperm X).
 Proof.
 rewrite /enum_fperm in_fset mem_pmap; apply/idP/mapP.
-  move=> supp_s; exists (val (val s)); last by rewrite /= !valK /= valK.
-  apply/enum_fmapP; split; first by move/fsubsetP: supp_s.
-  move=> x /codommP [x' Px']; move/fsubsetP: supp_s; apply.
+  move=> finsupp_s; exists (val (val s)); last by rewrite /= !valK /= valK.
+  apply/enum_fmapP; split; first by move/fsubsetP: finsupp_s.
+  move=> x /codommP [x' Px']; move/fsubsetP: finsupp_s; apply.
   have <- : s x' = x by rewrite /appf Px'.
-  by rewrite fperm_supp /supp mem_domm Px'.
+  by rewrite fperm_finsupp /finsupp mem_domm Px'.
 move=> [s' Ps' Pss']; case/enum_fmapP: Ps' => /fsubsetP.
 move: Pss' => /=; case: insubP => //= ? _ <-.
 by case: insubP => //= ? _ <- [] <-.
@@ -572,3 +568,30 @@ exact: fperm_inj.
 Qed.
 
 End Trans.
+
+#[deprecated(since="extructures 0.6.0", note="use imfset_finsupp instead")]
+Notation imfset_supp := imfset_finsupp (only parsing).
+#[deprecated(since="extructures 0.6.0", note="use imfset_finsuppS instead")]
+Notation imfset_suppS := imfset_finsuppS (only parsing).
+#[deprecated(since="extructures 0.6.0", note="use fperm_finsupp instead")]
+Notation fperm_supp := fperm_finsupp (only parsing).
+#[deprecated(since="extructures 0.6.0", note="use imfset_finsupp_sub instead")]
+Notation imfset_supp_sub := imfset_finsupp_sub (only parsing).
+#[deprecated(since="extructures 0.6.0", note="use finsupp1 instead")]
+Notation supp1 := finsupp1 (only parsing).
+#[deprecated(since="extructures 0.6.0", note="use finsupp_eq0 instead")]
+Notation supp_eq0 := finsupp_eq0 (only parsing).
+#[deprecated(since="extructures 0.6.0", note="use finsupp_fperm instead")]
+Notation supp_fperm := finsupp_fperm (only parsing).
+#[deprecated(since="extructures 0.6.0", note="use finsupp_inv instead")]
+Notation supp_inv := finsupp_inv (only parsing).
+#[deprecated(since="extructures 0.6.0", note="use fperm_finsuppV instead")]
+Notation fperm_suppV := fperm_finsuppV (only parsing).
+#[deprecated(since="extructures 0.6.0", note="use finsupp_mul instead")]
+Notation supp_mul := finsupp_mul (only parsing).
+#[deprecated(since="extructures 0.6.0", note="use finsuppJ instead")]
+Notation suppJ := finsuppJ (only parsing).
+#[deprecated(since="extructures 0.6.0", note="use finsupp_fperm2 instead")]
+Notation supp_fperm2 := finsupp_fperm2 (only parsing).
+#[deprecated(since="extructures 0.6.0", note="use fsubset_finsupp_fperm2 instead")]
+Notation fsubset_supp_fperm2 := fsubset_finsupp_fperm2 (only parsing).
